\documentclass[a4paper, 12pt]{scrartcl} 
\usepackage[english]{babel}
\usepackage[utf8]{inputenc}
\usepackage[T1]{fontenc}
\usepackage{ae,aecompl}

\usepackage{amsmath,amssymb,amstext}
\usepackage{psfrag}
\usepackage{float}
\usepackage[automark]{scrlayer-scrpage}

\usepackage{ifpdf}
\ifpdf
\usepackage[pdftex]{graphicx}
\usepackage{caption}
\usepackage{subcaption}
\pdfcompresslevel=9
\usepackage[pdftex=true, backref, pagebackref=false, colorlinks=true, bookmarks=true, bookmarksopen=false, bookmarksnumbered=false, pdfpagemode=None]{hyperref}
\DeclareGraphicsExtensions{.pdf}
\fi

\hypersetup{
pdftitle={}, 
pdfauthor={}, 
pdfsubject={}, 
pdfcreator={Accomplished with LaTeX2e and pdfLaTeX with hyperref-package.}, 
pdfproducer={}, 
pdfkeywords={} 
}
\newcommand{\mygraphics}[3]{
\begin{center}
\includegraphics[width=#1, keepaspectratio=true]{#2} \\
\textbf{#3}
\end{center}
}
\pagestyle{scrheadings}

\begin{document}
\section{Description Lab 1}

\subsection{Task 1}
\subsubsection{Subtask 1a}
Insert $x_w = v_w = \frac{dv_w}{dt} = i_A = 0$ into equation 3 of the mathematical model. \\
\begin{equation}
	\frac{dv_w}{dt} = 0 = \frac{1}{m_w + m_s(1-\cos(\phi)^2)} (m_s l \omega^2 \sin(\phi) - m_s g \sin(\phi) \cos(\phi))
\end{equation}
\begin{equation}
	m_s l \omega^2 \sin(\phi) = m_s g \sin(\phi) \cos(\phi)
\end{equation}
\begin{equation}
	l \omega^2 = g \cos(\phi)
\end{equation}
Than change the fourth equation of the mathematical model to get the form $\dot{\omega}(t) = p_1 f1(\phi(t), \omega(t), \dot{\omega}(t))$.
\begin{equation}
	\frac{d\omega}{dt} = \frac{1}{l\left(1-\frac{m_s}{m_w + m_s} \cos(\phi)^2\right)} \left( g \sin(\phi) - \frac{m_s}{m_w + m_s} \underbrace{l \omega^2}_{g \cos(\phi)} \sin(\phi) \cos(\phi) \right)
\end{equation}
\begin{equation}
	\frac{d\omega}{dt} = \frac{1}{l\left(1-\frac{m_s}{m_w + m_s} \cos(\phi)^2\right)} \left( g \sin(\phi) \left(1-\frac{m_s}{m_w + m_s} \cos(\phi)^2\right) \right)
\end{equation}
\begin{equation}
	\frac{d\omega}{dt} = \frac{g}{l} \sin(\phi)
\end{equation}
\subsubsection{Subtask 1b}
\subsubsection{Subtask 1c}
\subsubsection{Subtask 1d}

\subsection{Task 2}
\subsubsection{Subtask 1a}
\begin{equation}
	\begin{aligned}
	\dot{\omega} - g\sin(\phi) 
	&= \frac{1}{\left(1-\frac{m_s}{m_w + m_s} \cos(\phi)^2\right)} \left( g \sin(\phi) -  \frac{\cos(\phi)F}{m_w + m_s} - \frac{m_s}{m_w + m_s} {l \omega^2} \sin(\phi) \cos(\phi) \right) - g\sin(\phi)\\
	&= \frac{1}{\left(1-\frac{m_s}{m_w + m_s} \cos(\phi)^2\right)} \left( -\frac{\cos(\phi)F}{m_w + m_s} - \frac{m_s}{m_w + m_s} {l \omega^2} \sin(\phi) \cos(\phi) +\frac{m_s}{m_w + m_s} g\cos(\phi)^2 \sin(\phi) \right)\\
	&= \frac{m_w + m_s}{m_w+ m_s\sin(\phi)^2} \left( -\frac{\cos(\phi)F}{m_w + m_s} - \frac{m_s}{m_w + m_s} {l \omega^2} \sin(\phi) \cos(\phi) +\frac{m_s}{m_w + m_s} g\cos(\phi)^2 \sin(\phi) \right)\\
	&= \frac{1}{m_w+ m_s\sin(\phi)^2} \left( -\cos(\phi)F - m_s {l \omega^2} \sin(\phi) \cos(\phi) +m_s g\cos(\phi)^2 \sin(\phi) \right)\\
	\end{aligned}
\end{equation}

\subsubsection{Subtask 1b}
\subsubsection{Subtask 1c}
\subsubsection{Subtask 1d}
\subsubsection{Subtask 1e}
\subsubsection{Subtask 1f}

\subsection{Task 3}

\end{document}